Fix init in examples

examples/counter/extraction/CameLIGOCounter.v
@@ -29,9 +29,7 @@ Module Counter.
   Definition operation := ActionBody.
   Definition storage := Z × address.
 
-  Definition init (ctx : ContractCallContext) (setup : Z * address) : option storage :=
-    let ctx_ := ctx in (* prevents optimisations from removing unused [ctx]  *)
-    Some setup.
+  Definition init (setup : Z * address) : option storage := Some setup.
 
   Inductive msg :=
   | Inc (_ : Z)
