examples/escrow/extraction/EscrowExtract.v
@@ -108,7 +108,7 @@ Module EscrowCameLIGOExtraction.
 
   Time Definition cameLIGO_escrow := Eval vm_compute in cameligo_escrow_prepared.
 
-  (* Redirect "../extraction/tests/extracted-code/cameligo-extract/EscrowExtract.mligo" *)
+  Redirect "../extraction/tests/extracted-code/cameligo-extract/EscrowExtract.mligo"
   MetaCoq Run (tmMsg cameLIGO_escrow).
 
 End EscrowCameLIGOExtraction.
@@ -241,14 +241,14 @@ Module EscrowLiquidityExtraction.
     ].
 
   Import MonadNotation.
+  
+  Time MetaCoq Run
+      (t <- liquidity_extraction_specialize PREFIX TT_remap_liquidity TT_rename_liquidity to_inline ESCROW_MODULE_LIQUIDITY ;;
+        tmDefinition ESCROW_MODULE_LIQUIDITY.(lmd_module_name) t
+      ).
 
-  (* Time MetaCoq Run *)
-  (*     (t <- liquidity_extraction_specialize PREFIX TT_remap_liquidity TT_rename_liquidity to_inline ESCROW_MODULE_LIQUIDITY ;; *)
-  (*       tmDefinition ESCROW_MODULE_LIQUIDITY.(lmd_module_name) t *)
-  (*     ). *)
-
-  (* (** We redirect the extraction result for later processing and compiling with the Liquidity compiler *) *)
-  (* Redirect "../extraction/tests/extracted-code/liquidity-extract/escrow.liq" *)
-  (* MetaCoq Run (tmMsg liquidity_escrow). *)
+  (* (** we redirect the extraction result for later processing and compiling with the Liquidity compiler *) *)
+  Redirect "../extraction/tests/extracted-code/liquidity-extract/escrow.liq"
+  MetaCoq Run (tmMsg liquidity_escrow).
 
 End EscrowLiquidityExtraction.
